gcd with working linear combinations

math/Artin2_1.dfy
@@ -1,6 +1,6 @@
 
 //!A signifies type invariance
-datatype Group<!A> = Group(elements: set<A>, identity: A, compose: (A,A) -> A)
+datatype Group<!A> = Group(elements: set<A>, identity: A, compose: (A,A) -> A, inverse: (A) -> A)
 
 predicate isIdentity<A>(g: Group<A>) {
     forall a :: a in g.elements ==> g.compose(a,g.identity) == a && g.compose(g.identity, a) == a
@@ -18,15 +18,36 @@ predicate commutativeComposition<A>(g: Group<A>) {
     forall a,b :: a in g.elements && b in g.elements ==> g.compose(a,b) == g.compose(b,a)
 }
 
+//problematic, aka recursive trigger, it generates new patterns that match the trigger
 predicate containsInverses<A>(g: Group<A>) {
     forall x :: x in g.elements ==> exists xbar :: xbar in g.elements && g.compose(x,xbar) == g.identity
+}
+predicate PleaseInstantiateMe<A>(x: A) {
+    true
+}
+
+//no longer blocks apowAddition, but doesn't help groupCompositionInverse
+// predicate containsInverses<A>(g: Group<A>) {
+//   forall x {:trigger PleaseInstantiateMe(x)} :: 
+//     PleaseInstantiateMe(x) && x in g.elements ==> 
+//     exists xbar :: 
+//       xbar in g.elements && g.compose(x,xbar) == g.identity
+// }
+predicate closedInverse<A>(g: Group<A>) {
+  forall x {:trigger g.inverse(x)} :: x in g.elements ==> g.inverse(x) in g.elements
+}
+
+predicate isInverse<A>(g: Group<A>) {
+  forall x {:trigger g.inverse(x)} :: x in g.elements ==> g.compose(x,g.inverse(x)) == g.identity && g.compose(g.inverse(x),x) == g.identity
 }
 
 predicate ValidGroup<A>(g: Group<A>) {
     g.identity in g.elements &&
     isIdentity(g) &&
     closedComposition(g) &&
-    associativeComposition(g) //&&
+    associativeComposition(g) &&
+    closedInverse(g) &&
+    isInverse(g)
     // containsInverses(g)
 }
 
@@ -35,8 +56,8 @@ predicate ValidSubGroup<A>(g: Group<A>, h: Group<A>) {
     g.identity in h.elements &&
     g.identity == h.identity &&
     g.compose == h.compose &&
-    closedComposition(h) &&
-    containsInverses(h)
+    closedComposition(h) //&&
+    // containsInverses(h)
 }
 
 predicate AbelianGroup<A>(g: Group<A>) {
@@ -45,15 +66,11 @@ predicate AbelianGroup<A>(g: Group<A>) {
 
 lemma {:verify true} groupCompositionInverse<A>(g: Group<A>, a: A, b: A, abar: A, bbar: A, abbar: A)
     requires ValidGroup(g)
-    requires containsInverses(g)
     requires a in g.elements
     requires b in g.elements
-    requires abar in g.elements
-    requires bbar in g.elements
-    requires abbar in g.elements
-    requires g.compose(a, abar) == g.identity
-    requires g.compose(b, bbar) == g.identity
-    requires g.compose(g.compose(a, b), abbar) == g.identity
+    requires g.inverse(a) == abar
+    requires g.inverse(b) == bbar
+    requires g.inverse(g.compose(a,b)) == abbar
     ensures abbar == g.compose(bbar, abar)
 {
     calc {
@@ -69,6 +86,7 @@ lemma {:verify true} groupCompositionInverse<A>(g: Group<A>, a: A, b: A, abar: A
     }
 }
 
+//apow is short for abstract power
 function apow<A>(g: Group, elem: A, n: nat): A
     requires elem in g.elements
 {
@@ -93,10 +111,8 @@ lemma apowClosed<A>(g: Group, elem: A, n: nat)
     requires g.identity in g.elements
     requires isIdentity(g)
     requires closedComposition(g)
-    ensures apow(g,elem, n) in g.elements
-{
-
-}
+    ensures apow(g, elem, n) in g.elements
+{}
 
 lemma {:verify true} apowAddition<A>(g: Group<A>, elem: A, n: nat, k: nat)
     requires elem in g.elements
@@ -107,12 +123,13 @@ lemma {:verify true} apowAddition<A>(g: Group<A>, elem: A, n: nat, k: nat)
     apowClosed(g, elem, k);
     if k == 0 {
         assert apow(g, elem, k) == g.identity;
-        assert g.compose(apow(g, elem, n), g.identity) == apow(g, elem, n+0);
+        assert g.compose(apow(g, elem, n), g.identity) == apow(g, elem, n+k);
     }else if n == 0 {
         assert apow(g, elem, n) == g.identity;
-        assert g.compose(g.identity, apow(g, elem, k)) == apow(g, elem, k+0);
+        assert g.compose(g.identity, apow(g, elem, k)) == apow(g, elem, n+k);
     }else{
         apowClosed(g, elem, n-1);
+        apowClosed(g, elem, n+k);
         calc {
             g.compose(apow(g, elem, n), apow(g, elem, k));
             g.compose(g.compose(elem, apow(g, elem, n-1)), apow(g, elem, k));
@@ -130,7 +147,7 @@ predicate CyclicGroupGeneratedBy<A(!new)>(g: Group, elem: A)
     exists n :: n == |g.elements| &&
         apow(g, elem, n) == g.identity &&
         (forall ns :: ns != n && apow(g, elem, ns) == g.identity ==> n < ns) &&
-        n != 0 && |g.elements| == n &&
+        n != 0 &&
         forall x :: x in g.elements && exists n :: apow(g, elem, n) == x
 }
 
@@ -138,7 +155,7 @@ lemma {:verify false} AllSubgroupsOfCyclicSubgroupsAreCyclic<A(!new)>(g: Group, 
     requires elem in g.elements
     requires CyclicGroupGeneratedBy(g, elem)
     requires ValidGroup(g)
-    requires h.elements < g.elements
+    requires h.elements <= g.elements
     requires ValidGroup(h)
     requires ValidSubGroup(g, h)
     ensures exists hx: A :: hx in h.elements && CyclicGroupGeneratedBy(h, hx)
