math/gcd.dfy
@@ -1,0 +1,417 @@
+
+module Math {
+    //imported from https://github.com/dafny-lang/dafny/blob/master/Test/dafny4/gcd.dfy
+    type pos = x: nat | 1 <= x witness 1
+    predicate IsFactor(p: pos, x: pos) {
+        exists q: pos ::  p * q == x
+    }
+
+    function Factors(x: pos): set<pos> {
+        set p: pos | p <= x  && IsFactor(p, x)  // error: set constructed must be finite
+    }
+
+    lemma FactorIsFactorOfLinearCombination(a: pos, b: pos, c: pos)
+        requires IsFactor(a, b)
+        requires IsFactor(a, c)
+        ensures forall x,y :: linearCombination(b,x,c,y) > 0 ==> IsFactor(a, linearCombination(b,x,c,y))
+    {
+       forall x,y | linearCombination(b,x,c,y) > 0 
+            ensures IsFactor(a, linearCombination(b,x,c,y))
+       {
+            var qq :| a*qq == c;
+            var ll :| a*ll == b;
+            calc {
+                linearCombination(b,x,c,y);
+                linearCombination(a*ll,x,a*qq,y);
+                prod(a*ll,x) + prod(a*qq,y);
+                == {reveal prod();}
+                prod(prod(a,ll),x) + prod(prod(a,qq),y);
+                == {prodAssociative(a,ll,x);}
+                prod(a, prod(ll,x)) + prod(prod(a,qq),y);
+                == {prodAssociative(a,qq,y);}
+                prod(a, prod(ll,x)) + prod(a,prod(qq,y));
+                == {prodDistributes(a, prod(ll,x), prod(qq,y));}
+                prod(a, prod(ll,x) +prod(qq,y));
+                == {reveal prod();}
+                a * (ll*x + qq*y);
+            }
+            assert (ll*x + qq*y) > 0;
+            assert a * (ll*x + qq*y) == linearCombination(b,x,c,y);
+            assert IsFactor(a, linearCombination(b,x,c,y));
+
+       } 
+    }
+
+    lemma FactorsHasAllFactors(x: pos)
+        ensures forall n :: n in Factors(x) <==> n in iset p: pos | IsFactor(p, x)
+    {
+    }
+
+    lemma FactorsContains1(x: pos)
+        ensures 1 in Factors(x)
+    {
+        assert 1 * x == x;
+    }
+
+    lemma FactorsContainsSelf(x: pos)
+        ensures x in Factors(x)
+    {
+        assert x * 1 == x;
+    }
+
+    function Max(s: set<pos>): pos
+        requires s != {}
+    {
+        MaxExists(s);
+        var x :| x in s && forall y :: y in s ==> y <= x;
+        x
+    }
+    lemma MaxExists(s: set<pos>)
+        requires s != {}
+        ensures exists x :: x in s && forall y :: y in s ==> y <= x
+    {
+        var x := FindMax(s);
+    }
+
+    function FindMax(s: set<pos>): (max: pos)
+        requires s != {}
+        ensures max in s && forall y :: y in s ==> y <= max
+    {
+        var x :| x in s;
+        if s == {x} then
+            x
+        else
+            var s' := s - {x};
+            assert s == s' + {x};
+            var y := FindMax(s');
+            if x < y then y else x
+    }
+
+    function Min(s: set<pos>): pos 
+        requires s != {}
+        ensures forall x | x in s :: Min(s) in s && Min(s) <= x
+    {
+        var x :| x in s;
+        if s == {x} then
+            x
+        else
+            var y := Min(s - {x});
+            assert forall z | z in s :: z == x || (z in (s - {x}) && y <= z);
+            if x < y then x else y
+    }
+
+    lemma WellOrderingPrinciple(s: iset<pos>)
+        requires s != iset{}
+        ensures exists min :: min in s && forall x | x in s && x != min :: min < x; 
+
+    function iMin(s: iset<pos>): pos
+        requires s != iset{}
+        ensures forall x | x in s && x != iMin(s) :: iMin(s) in s ==> iMin(s) < x
+    {
+        WellOrderingPrinciple(s);
+        var min :| min in s && forall x | x in s && x != min :: min < x; 
+        min
+    }
+
+
+    function Gcd(x: pos, y: pos): pos {
+        var common := Factors(x) * Factors(y);
+        assert 1 in common by {
+            FactorsContains1(x);
+            FactorsContains1(y);
+        }
+        Max(common)
+    }
+
+    lemma AboutGcd(x: pos, y: pos)
+        ensures IsFactor(Gcd(x, y), x)
+        ensures IsFactor(Gcd(x, y), y)
+        ensures forall p: pos :: IsFactor(p, x) && IsFactor(p, y) ==> p <= Gcd(x, y)
+    {
+        forall p: pos | IsFactor(p, x) && IsFactor(p, y)
+            ensures p <= Gcd(x, y)
+        {
+            assert p in Factors(x) * Factors(y);
+        }
+    }
+
+    lemma GcdSymmetric(x: pos, y: pos)
+        ensures Gcd(x, y) == Gcd(y, x)
+    {
+        assert Factors(x) * Factors(y) == Factors(y) * Factors(x);
+    }
+
+    lemma GcdIdempotent(x: pos)
+        ensures Gcd(x, x) == x
+    {
+        FactorsContainsSelf(x);
+        assert x in Factors(x) * Factors(x);
+    }
+
+    lemma GcdSubtract(x: pos, y: pos)
+        requires x < y
+        ensures Gcd(x, y) == Gcd(x, y - x)
+    {
+        var p := Gcd(x, y);
+
+        // By the definition of `Gcd`, we know that p is a factor of both x and y,
+        // We now show that p is also a factor of y - x.
+        assert IsFactor(p, y - x) by {
+            var a :| p * a == x;
+            var b :| p * b == y;
+            calc {
+            y - x;
+            ==
+            p * b - p * a;
+            ==
+            p * (b - a);
+            }
+        }
+
+        // Hence, p is a common factor of x and y - x
+        var common := Factors(x) * Factors(y - x);
+        assert p in common;
+
+        // It remains to show that, among the common factors of x and
+        // y - x, p is the greatest
+        forall q | q in common
+            ensures q <= p
+        {
+            // q is a factor of both x and y - x, so a and b exist:
+            var a :| q * a == x;
+            var b :| q * b == y - x;
+            assert IsFactor(q, y) by {
+            calc {
+                y;
+            ==
+                x + (y - x);
+            ==
+                q * a + q * b;
+            ==
+                q * (a + b);
+            }
+            }
+            // We just showed that q is a common factor of x and y.
+            assert q in Factors(x) * Factors(y);
+            // By the definition of Gcd(x, y), we then have that q <= p.
+        }
+    }
+
+    method EuclidGcd(X: pos, Y: pos) returns (gcd: pos)
+        ensures gcd == Gcd(X, Y)
+    {
+        var x: pos, y: pos := X, Y;
+        while
+            invariant Gcd(x, y) == Gcd(X, Y)
+            decreases x + y
+        {
+            case x < y =>
+            GcdSubtract(x, y);
+            y := y - x;
+            case y < x =>
+            calc {
+                Gcd(x, y);
+            ==  { GcdSymmetric(x, y); }
+                Gcd(y, x);
+            ==  { GcdSubtract(y, x); }
+                Gcd(y, x - y);
+            ==  { GcdSymmetric(y, x - y); }
+                Gcd(x - y, y);
+            }
+            x := x - y;
+        }
+        GcdIdempotent(x);
+        return x;
+    }
+
+    function linearCombination(a: int, x: int, b: int, y: int): int {
+        // a*x + b*y
+        prod(a,x) + prod(b,y)
+    }
+
+    function combinationSet(a: pos, b: pos): set<pos> 
+    {
+        // set x: nat,y: nat | 0 <= x <= a && 0 <= y <= b && a*x+b*y > 0 :: a*x+b*y
+        set x: int,y: int | 0 <= x <= a && 0 <= y <= b && linearCombination(a,x,b,y) > 0 :: linearCombination(a,x,b,y)
+    }
+
+    function icombinationSet(a: pos, b: pos): iset<pos> 
+    {
+        iset x: int,y: int | linearCombination(a,x,b,y) > 0 :: linearCombination(a,x,b,y)
+        // iset x: int,y: int | a*x+b*y > 0 :: a*x+b*y
+    }
+
+    function {:opaque} prod(x: int, y: int): int {
+        x * y
+    }
+
+    function divAdd(b: int, a: int, c: int): int {
+        prod(b,a) + c
+    }
+
+    lemma {:verify true} DivisionAlgorithm(a: pos, b: pos)
+        requires a != 0
+        ensures exists q: nat,r:nat :: b == divAdd(q,a,r) && 0 <= r < a
+    {
+        var r := b%a;
+        var q := b/a;
+        reveal prod();
+        assert b == divAdd(q,a,r);
+    }
+
+    lemma prodAssociative(a: int, b: int, c: int)
+        ensures prod(prod(a,b),c) == prod(a, prod(b,c))
+    {
+        reveal prod();
+    }
+
+    lemma prodCommutes(a: int, b: int)
+        ensures prod(a,b) == prod(b,a)
+    {
+        reveal prod();
+    }
+
+    lemma prodCommutesThree(a: int, b: int, c: int) 
+        ensures prod(a, prod(b, c)) == prod(b, prod(a, c))
+    {
+        reveal prod();
+    }
+
+    lemma prodDistributes(a: int, b: int, c: int)
+        ensures prod(a, b + c) == prod(a,b) + prod(a,c)
+    {
+        reveal prod();
+    }
+
+    lemma prodDistributesMinus(a: int, b: int, c: int)
+        ensures prod(a, b - c) == prod(a,b) - prod(a,c)
+    {
+        reveal prod();
+    }
+
+    lemma prodIdentity(a: int)
+        ensures a == prod(a, 1)
+        ensures a == prod(1, a)
+    {
+        reveal prod();
+    }
+    lemma prodNegative(a: int, b: int)
+        ensures -prod(a,b) == prod(-1, prod(a,b))
+    {
+        reveal prod();
+    }
+
+    lemma linearCombinationOfPosisPos(a: pos, b: pos)
+        ensures linearCombination(a,a,b,b) > 0;
+    {
+        assert a > 0;
+        assert b > 0;
+        calc {
+            linearCombination(a,a,b,b);
+            prod(a,a) + prod(b,b);
+            == {reveal prod();}
+            a*a + b * b;
+        }
+    }
+    
+    lemma DivAddZero(a: int, q: int, d: int)
+        requires a > 0
+        requires d > 0
+        requires a == divAdd(q,d,0)
+        ensures IsFactor(d,a)
+    {
+        reveal prod();
+        calc {
+            divAdd(q,d, 0);
+            prod(q,d)  + 0;
+            prod(q,d);
+            q*d;
+            a;
+        }
+        assert d*q == a;
+        assert IsFactor(d,a);
+    }
+    
+    lemma {:verify true} GcdLinearCombination(a: pos, b: pos)
+        ensures exists x,y :: Gcd(a,b) == linearCombination(a,x,b,y)
+    {
+        AboutGcd(a,b);
+        var S := icombinationSet(a,b);
+        linearCombinationOfPosisPos(a,b);
+        assert linearCombination(a,a,b,b) > 0 && linearCombination(a,a,b,b) in S;
+        var d := iMin(S);
+        assert d in S;
+        ghost var s,t :| d == linearCombination(a,s,b,t);
+        DivisionAlgorithm(d,a);
+        ghost var q,r :| a == divAdd(q,d,r) &&  0 <= r < d;
+        if r > 0 {
+            calc {
+                r;
+                a - prod(q,d);
+                a - prod(q, linearCombination(a,s,b,t));
+                a - prod(q, prod(a,s)+prod(b,t));
+                == {prodDistributes(q, prod(a,s), prod(b,t));}
+                a - (prod(q, prod(a,s))+prod(q, prod(b,t)));
+                == {prodCommutesThree(q,a,s);}
+                a - (prod(a, prod(q,s))+prod(q, prod(b,t)));
+                == {prodCommutesThree(q,b,t);}
+                a - prod(a, prod(q,s)) - prod(b, prod(q,t));
+                =={ prodIdentity(a);}
+                prod(a,1) - prod(a, prod(q,s)) - prod(b, prod(q,t));
+                == { prodDistributesMinus(a, 1, prod(q,s));}
+                prod(a,1 - prod(q,s)) - prod(b, prod(q,t));
+                prod(a,1 - prod(q,s)) - prod(b, prod(q,t));
+                == {prodNegative(b, prod(q,t));}
+                prod(a,1 - prod(q,s)) + prod(-1,prod(b, prod(q,t)));
+                == {prodCommutesThree(-1,b, prod(q,t));}
+                prod(a,1 - prod(q,s)) + prod(b, prod(-1, prod(q,t)));
+                linearCombination(a, 1- prod(q,s), b, prod(-1, prod(q,t)));
+            }
+            assert r in icombinationSet(a,b);
+            assert r < d;
+            assert d < r;
+            assert false;
+        }
+        assert r == 0;
+        assert a == divAdd(q,d,0);
+      
+        DivisionAlgorithm(d,b);
+        ghost var l,k :| b == divAdd(l,d,k) &&  0 <= k < d;
+        if k > 0 {
+            calc {
+                k;
+                b - prod(l,d);
+                b - prod(l, linearCombination(a,s,b,t));
+                b - prod(l, prod(a,s)+prod(b,t));
+                == {prodDistributes(l, prod(a,s), prod(b,t));}
+                b - (prod(l, prod(a,s))+prod(l, prod(b,t)));
+                == {prodCommutesThree(l,a,s);}
+                b - (prod(a, prod(l,s))+prod(l, prod(b,t)));
+                == {prodCommutesThree(l,b,t);}
+                b - prod(a, prod(l,s)) - prod(b, prod(l,t));
+                - prod(a, prod(l,s)) + b - prod(b, prod(l,t));
+                == {prodNegative(a, prod(l,s));}
+                prod(-1, prod(a, prod(l,s))) + b - prod(b, prod(l,t));
+                == {prodCommutesThree(-1, a, prod(l,s));}
+                prod(a, prod(-1, prod(l,s))) + b - prod(b, prod(l,t));
+                =={ prodIdentity(b);}
+                prod(a, prod(-1, prod(l,s))) + prod(b,1) - prod(b, prod(l,t));
+                == { prodDistributesMinus(b, 1, prod(l,t));}
+                prod(a, prod(-1, prod(l,s))) + prod(b,1 - prod(l,t));
+                linearCombination(a, prod(-1, prod(l,s)), b, 1 - prod(l,t));
+            }
+            assert k in icombinationSet(a,b);
+            assert k < d;
+            assert d < k;
+            assert false;
+        }
+        assert k == 0;
+        assert b == divAdd(l,d,0);
+
+        DivAddZero(a,q,d);
+        DivAddZero(b,l,d);
+        var c := Gcd(a,b);
+        FactorIsFactorOfLinearCombination(c,a,b);
+    }
+
+}
